JamesC - dropped general pattern matching in favour of cases

isabelle/Chapter13_1_Language.thy
@@ -11,26 +11,25 @@ datatype type =
 | Sum type type
 
 datatype patn =
-  Wild
-| PVar
-| PTriv
-| PPair patn patn
-| PInL patn
-| PInR patn
+  PTriv
+| PPair
+| PInL
+| PInR
+| PZero
+| PSucc
 
 primrec vars_count :: "patn => nat"
-where "vars_count Wild = 0"
-    | "vars_count PVar = 1"
-    | "vars_count PTriv = 0"
-    | "vars_count (PPair p1 p2) = vars_count p1 + vars_count p2"
-    | "vars_count (PInL p) = vars_count p"
-    | "vars_count (PInR p) = vars_count p"
+where "vars_count PTriv = 0"
+    | "vars_count PPair = 2"
+    | "vars_count PInL = 1"
+    | "vars_count PInR = 1"
+    | "vars_count PZero = 0"
+    | "vars_count PSucc = 1"
 
 datatype expr = 
   Var nat 
 | Zero
 | Succ expr
-| IsZ expr expr expr
 | Lam type expr
 | Ap expr expr
 | Fix type expr
@@ -41,7 +40,7 @@ datatype expr =
 | Abort type expr
 | InL type type expr
 | InR type type expr
-| Match expr type "rule list"
+| Case expr type "rule list"
 and rule = Rule patn expr
 
 definition redr_set :: "nat set => nat set"
@@ -89,7 +88,6 @@ primrec free_vars :: "expr => nat set"
 where "free_vars (Var v) = {v}"
     | "free_vars Zero = {}"
     | "free_vars (Succ e) = free_vars e"
-    | "free_vars (IsZ e0 e1 et) = free_vars e0 Un free_vars et Un redr_set (free_vars e1)"
     | "free_vars (Lam t b) = redr_set (free_vars b)"
     | "free_vars (Ap e1 e2) = free_vars e1 Un free_vars e2"
     | "free_vars (Fix t b) = redr_set (free_vars b)"
@@ -100,7 +98,7 @@ where "free_vars (Var v) = {v}"
     | "free_vars (Abort t e) = free_vars e"
     | "free_vars (InL t t' e) = free_vars e"
     | "free_vars (InR t t' e) = free_vars e"
-    | "free_vars (Match e t rs) = free_vars e Un free_vars_rules rs"
+    | "free_vars (Case e t rs) = free_vars e Un free_vars_rules rs"
     | "free_vars_rules Nil = {}"
     | "free_vars_rules (r # rs) = free_vars_rule r Un free_vars_rules rs"    
     | "free_vars_rule (Rule p e) = redr_set_by (vars_count p) (free_vars e)"
@@ -117,7 +115,6 @@ primrec incr_from :: "nat => expr => expr"
 where "incr_from n (Var v) = Var (incr n v)"
     | "incr_from n Zero = Zero"
     | "incr_from n (Succ e) = Succ (incr_from n e)"
-    | "incr_from n (IsZ e0 e1 et) = IsZ (incr_from n e0) (incr_from (Suc n) e1) (incr_from n et)"
     | "incr_from n (Lam t b) = Lam t (incr_from (Suc n) b)"
     | "incr_from n (Ap e1 e2) = Ap (incr_from n e1) (incr_from n e2)"
     | "incr_from n (Fix t b) = Fix t (incr_from (Suc n) b)"
@@ -128,7 +125,7 @@ where "incr_from n (Var v) = Var (incr n v)"
     | "incr_from n (Abort t e) = Abort t (incr_from n e)"
     | "incr_from n (InL t t' e) = InL t t' (incr_from n e)"
     | "incr_from n (InR t t' e) = InR t t' (incr_from n e)"
-    | "incr_from n (Match e t rs) = Match (incr_from n e) t (incr_from_rules n rs)"
+    | "incr_from n (Case e t rs) = Case (incr_from n e) t (incr_from_rules n rs)"
     | "incr_from_rules n Nil = Nil"
     | "incr_from_rules n (r # rs) = incr_from_rule n r # incr_from_rules n rs"    
     | "incr_from_rule n (Rule p e) = Rule p (incr_from (n + vars_count p) e)"
@@ -150,8 +147,7 @@ proof (auto simp add: incr_def)
     ultimately show "x : incr n ` redr_set xs" by simp
   qed
 next
-  fix xa
-  show "Suc xa : xs ==> xa < n ==> Suc xa : incr (Suc n) ` xs" by (auto simp add: incr_def)
+  show "!!xa. Suc xa : xs ==> xa < n ==> Suc xa : incr (Suc n) ` xs" by (auto simp add: incr_def)
 next 
   fix xa
   assume "Suc xa : xs"
@@ -187,7 +183,6 @@ primrec sub_from :: "nat => expr => expr"
 where "sub_from n (Var v) = Var (if v < n then v else if v = n then undefined else v - 1)"
     | "sub_from n Zero = Zero"
     | "sub_from n (Succ e) = Succ (sub_from n e)"
-    | "sub_from n (IsZ e0 e1 et) = IsZ (sub_from n e0) (sub_from (Suc n) e1) (sub_from n et)"
     | "sub_from n (Lam t b) = Lam t (sub_from (Suc n) b)"
     | "sub_from n (Ap e1 e2) = Ap (sub_from n e1) (sub_from n e2)"
     | "sub_from n (Fix t b) = Fix t (sub_from (Suc n) b)"
@@ -198,7 +193,7 @@ where "sub_from n (Var v) = Var (if v < n then v else if v = n then undefined el
     | "sub_from n (Abort t e) = Abort t (sub_from n e)"
     | "sub_from n (InL t t' e) = InL t t' (sub_from n e)"
     | "sub_from n (InR t t' e) = InR t t' (sub_from n e)"
-    | "sub_from n (Match e t rs) = Match (sub_from n e) t (sub_from_rules n rs)"
+    | "sub_from n (Case e t rs) = Case (sub_from n e) t (sub_from_rules n rs)"
     | "sub_from_rules n Nil = Nil"
     | "sub_from_rules n (r # rs) = sub_from_rule n r # sub_from_rules n rs"    
     | "sub_from_rule n (Rule p e) = Rule p (sub_from (n + vars_count p) e)"
@@ -212,7 +207,6 @@ primrec subst :: "expr => expr => nat => expr"
 where "subst (Var v) e x = (if v = x then e else Var v)"
     | "subst Zero e x = Zero"
     | "subst (Succ n) e x = Succ (subst n e x)"
-    | "subst (IsZ e0 e1 et) e x = IsZ (subst e0 e x) (subst e1 (incr_from 0 e) (Suc x)) (subst et e x)"
     | "subst (Lam t b) e x = Lam t (subst b (incr_from 0 e) (Suc x))"
     | "subst (Ap e1 e2) e x = Ap (subst e1 e x) (subst e2 e x)"
     | "subst (Fix t b) e x = Fix t (subst b (incr_from 0 e) (Suc x))"
@@ -223,7 +217,7 @@ where "subst (Var v) e x = (if v = x then e else Var v)"
     | "subst (Abort t n) e x = Abort t (subst n e x)"
     | "subst (InL t t' n) e x = InL t t' (subst n e x)"
     | "subst (InR t t' n) e x = InR t t' (subst n e x)"
-    | "subst (Match ec t rs) e x = Match (subst ec e x) t (subst_rules rs e x)"
+    | "subst (Case ec t rs) e x = Case (subst ec e x) t (subst_rules rs e x)"
     | "subst_rules Nil e x = Nil"
     | "subst_rules (r # rs) e x = subst_rule r e x # subst_rules rs e x"
     | "subst_rule (Rule p b) e x = Rule p (subst b (incr_by (vars_count p) e) (x + vars_count p))"
