isabelle/Chapter13_3_PatternMatching.thy
@@ -6,7 +6,6 @@ fun is_val :: "expr => bool"
 where "is_val (Var v) = False"
     | "is_val Zero = True"
     | "is_val (Succ n) = is_val n"
-    | "is_val (IsZ e0 e1 et) = False"
     | "is_val (Lam t b) = True"
     | "is_val (Ap e1 e2) = False"
     | "is_val (Fix t b) = False"
@@ -17,7 +16,7 @@ where "is_val (Var v) = False"
     | "is_val (Abort t e) = False"
     | "is_val (InL t t' e) = is_val e"
     | "is_val (InR t t' e) = is_val e"
-    | "is_val (Match e t rs) = False"
+    | "is_val (Case e t rs) = False"
 
 lemma canonical_nat: "typecheck env e Nat ==> is_val e ==> e = Zero | (EX v. typecheck env v Nat & is_val v & e = Succ v)"
 by (induction e, auto)
@@ -39,153 +38,82 @@ lemma canonical_sum: "typecheck env e (Sum t1 t2) ==> is_val e ==>
 by (induction e, auto)
 
 inductive matches :: "expr list => patn => expr => bool"
-where mtchw [simp]: "matches [] Wild e"
-    | mtchv [simp]: "matches [e] PVar e"
-    | mtcht [simp]: "matches [] PTriv Triv"
-    | mtchp [simp]: "matches s1 p1 e1 ==> matches s2 p2 e2 ==> matches (s1 @ s2) (PPair p1 p2) (Pair e1 e2)"
-    | mtchl [simp]: "matches s p e ==> matches s (PInL p) (InL t t' e)"
-    | mtchr [simp]: "matches s p e ==> matches s (PInR p) (InR t t' e)"
+where mtcht [simp]: "matches [] PTriv Triv"
+    | mtchp [simp]: "matches [e1, e2] PPair (Pair e1 e2)"
+    | mtchl [simp]: "matches [e] PInL (InL t t' e)"
+    | mtchr [simp]: "matches [e] PInR (InR t t' e)"
+    | mtchz [simp]: "matches [] PZero Zero"
+    | mtchs [simp]: "matches [e] PSucc (Succ e)"
 
-inductive_cases [elim!]: "matches s Wild e"
-inductive_cases [elim!]: "matches s PVar e"
 inductive_cases [elim!]: "matches s PTriv e"
-inductive_cases [elim!]: "matches s (PPair x y) e"
-inductive_cases [elim!]: "matches s (PInL x) e"
-inductive_cases [elim!]: "matches s (PInR x) e"
+inductive_cases [elim!]: "matches s PPair e"
+inductive_cases [elim!]: "matches s PInL e"
+inductive_cases [elim!]: "matches s PInR e"
+inductive_cases [elim!]: "matches s PZero e"
+inductive_cases [elim!]: "matches s PSucc e"
 
 inductive no_match :: "expr => patn => bool"
-where [simp]: "no_match e1 p1 ==> no_match (Pair e1 e2) (PPair p1 p2)"
-    | [simp]: "no_match e2 p2 ==> no_match (Pair e1 e2) (PPair p1 p2)"
-    | [simp]: "no_match (InL t t' e) (PInR p)"
-    | [simp]: "no_match e p ==> no_match (InL t t' e) (PInL p)"
-    | [simp]: "no_match (InR t t' e) (PInL p)"
-    | [simp]: "no_match e p ==> no_match (InR t t' e) (PInR p)"
+where [simp]: "no_match (InL t t' e) PInR"
+    | [simp]: "no_match (InR t t' e) PInL"
+    | [simp]: "no_match Zero PSucc"
+    | [simp]: "no_match (Succ e) PZero"
 
-lemma [simp]: "no_match (Pair e1 e2) (PPair p1 p2) ==> no_match e1 p1 | no_match e2 p2"
-by (auto, induction "Pair e1 e2" "PPair p1 p2" rule: no_match.induct, auto)
-
-lemma [simp]: "no_match (InL t t' e) (PInL p) = no_match e p"
-by (auto, induction "InL t t' e" "PInL p" rule: no_match.induct, simp)
-
-lemma [simp]: "no_match (InR t t' e) (PInR p) = no_match e p"
-by (auto, induction "InR t t' e" "PInR p" rule: no_match.induct, simp)
-
-lemma [simp]: "matches s p e ==> ~ no_match e p"
-proof (induction s p e rule: matches.induct)
-case (mtchw e)
-  thus ?case by (auto, induction e Wild rule: no_match.induct)
-next case (mtchv e)
-  thus ?case by (auto, induction e PVar rule: no_match.induct)
-next case mtcht
-  thus ?case by (auto, induction Triv PTriv rule: no_match.induct)
-next case (mtchp s1 p1 e1 s2 p2 e2)
-  thus ?case
-  proof auto 
-    assume "no_match (Pair e1 e2) (PPair p1 p2)"
-       and "matches s1 p1 e1"
-       and "matches s2 p2 e2"
-       and "~ no_match e1 p1"
-       and "~ no_match e2 p2"
-    thus False by (induction "Pair e1 e2" "PPair p1 p2" rule: no_match.induct, simp_all)
+lemma [simp]: "(~ no_match e p) = matches s p e"
+proof auto
+  show "~ no_match e p ==> matches s p e" by simp sorry
+next 
+  show "matches s p e ==> no_match e p ==> False"
+  proof (induction s p e rule: matches.induct)
+  case mtcht
+    thus ?case by (induction Triv PTriv rule: no_match.induct)
+  next case (mtchp e1 e2)
+    thus ?case by (induction "Pair e1 e2" PPair rule: no_match.induct)
+  next case (mtchl e t t')
+    thus ?case by (induction "InL t t' e" PInL rule: no_match.induct)
+  next case (mtchr e t t')
+    thus ?case by (induction "InR t t' e" PInR rule: no_match.induct)
+  next case mtchz
+    thus ?case by (induction Zero PZero rule: no_match.induct)
+  next case (mtchs e)
+    thus ?case by (induction "Succ e" PSucc rule: no_match.induct)
   qed
-next case mtchl
-  thus ?case by simp 
-next case (mtchr s p e)
-  thus ?case by simp 
 qed
 
 lemma [simp]: "types_from_pat p t ts ==> typecheck env e t ==> is_val e ==> (EX s. typecheck_subst env s ts & matches s p e) | no_match e p"
 proof (induction p t ts arbitrary: e rule: types_from_pat.induct)
-case tpwld
-  have "typecheck_subst env [] [] & matches [] Wild e" by simp
-  hence "EX s. typecheck_subst env s [] & matches s Wild e" by (rule exI)
-  thus ?case by simp
-next case (tpvar t)
-  hence "typecheck_subst env [e] [t] & matches [e] PVar e" by simp
-  hence "EX s. typecheck_subst env s [t] & matches s PVar e" by (rule exI)
-  thus ?case by simp
-next case tptrv
+case tptrv
   hence "e = Triv" by (simp add: canonical_unit)
-  hence "typecheck_subst env [] [] & matches [] PTriv e" by simp
-  hence "EX s. typecheck_subst env s [] \<and> matches s PTriv e" by (rule exI)
-  thus ?case by simp
-next case (tppar p1 t1 ts1 p2 t2 ts2)
+  thus ?case by simp sorry
+next case (tppar t1 t2)
   hence "(EX e1 e2. e = Pair e1 e2 & typecheck env e1 t1 & typecheck env e2 t2 & is_val e1 & is_val e2)" by (simp add: canonical_prod)
-  with tppar show ?case
-  proof auto
-    fix e1 e2 s1 s2
-    assume "!!e. typecheck env e t1 ==> is_val e ==> (EX s. typecheck_subst env s ts1 & matches s p1 e) | no_match e p1"
-       and "typecheck env e1 t1"
-       and "is_val e1"
-    hence A: "(EX s. typecheck_subst env s ts1 & matches s p1 e1) | no_match e1 p1" by auto
-    assume "!!e. typecheck env e t2 ==> is_val e ==> (EX s. typecheck_subst env s ts2 & matches s p2 e) | no_match e p2"
-       and "typecheck env e2 t2"
-       and "is_val e2"
-    hence B: "(EX s. typecheck_subst env s ts2 & matches s p2 e2) | no_match e2 p2" by auto
-    assume C: "~ no_match (Pair e1 e2) (PPair p1 p2)"
-    from A C have "EX s. typecheck_subst env s ts1 & matches s p1 e1" by auto
-    moreover from B C have "EX s. typecheck_subst env s ts2 & matches s p2 e2" by auto
-    ultimately show "EX s. typecheck_subst env s (ts1 @ ts2) & matches s (PPair p1 p2) (Pair e1 e2)"
-    proof auto
-      fix s1 s2
-      assume "typecheck_subst env s1 ts1"
-         and "matches s1 p1 e1"
-         and "typecheck_subst env s2 ts2"
-         and "matches s2 p2 e2"
-      hence "typecheck_subst env (s1 @ s2) (ts1 @ ts2) & matches (s1 @ s2) (PPair p1 p2) (Pair e1 e2)" by simp
-      thus "EX s. typecheck_subst env s (ts1 @ ts2) & matches s (PPair p1 p2) (Pair e1 e2)" by auto
-    qed
-  qed
-next case (tpinl p t1 ts t2)
+  with tppar show ?case by auto sorry
+next case (tpinl t1 t2)
   from tpinl have "(EX e'. e = InL t1 t2 e' & is_val e' & typecheck env e' t1) | (EX e'. e = InR t1 t2 e' & is_val e' & typecheck env e' t2)" by (simp add: canonical_sum)
   with tpinl show ?case
   proof (cases "EX e'. e = InL t1 t2 e'", auto)
     fix e'
-    assume "!!e. typecheck env e t1 ==> is_val e ==> (EX s. typecheck_subst env s ts & matches s p e) | no_match e p"
-       and "~ no_match e' p"
-       and "is_val e'"
-       and "typecheck env e' t1"
-    hence "EX s. typecheck_subst env s ts & matches s p e'" by auto
-    thus "EX s. typecheck_subst env s ts & matches s (PInL p) (InL t1 t2 e')" by auto
+    show "EX s. typecheck_subst env s [t1] & matches s PInL (InL t1 t2 e')" by auto sorry
   qed
-next case (tpinr p t2 ts t1)
+next case (tpinr t1 t2)
   from tpinr have "(EX e'. e = InL t1 t2 e' & is_val e' & typecheck env e' t1) | (EX e'. e = InR t1 t2 e' & is_val e' & typecheck env e' t2)" by (simp add: canonical_sum)
   with tpinr show ?case
   proof (cases "EX e'. e = InR t1 t2 e'", auto)
     fix e'
-    assume "!!e. typecheck env e t2 ==> is_val e ==> (EX s. typecheck_subst env s ts & matches s p e) | no_match e p"
-       and "~ no_match e' p"
-       and "is_val e'"
+    assume "\<not> no_match (InR t1 t2 e') PInR" 
+       and "is_val e'" 
        and "typecheck env e' t2"
-    hence "EX s. typecheck_subst env s ts & matches s p e'" by auto
-    thus "EX s. typecheck_subst env s ts & matches s (PInR p) (InR t1 t2 e')" by auto
+    show "EX s. typecheck_subst env s [t2] & matches s PInR (InR t1 t2 e')" by auto sorry
   qed
+next case tpzer
+  hence "e = Zero | (EX v. typecheck env v Nat & is_val v & e = Succ v)" by (simp add: canonical_nat)
+  thus ?case by simp sorry
+next case tpsuc
+  hence "e = Zero | (EX v. typecheck env v Nat & is_val v & e = Succ v)" by (simp add: canonical_nat)
+  show ?case by auto sorry
 qed
 
 lemma [simp]: "matches s p e ==> matches s' p e ==> s = s'"
-proof (induction s p e arbitrary: s' rule: matches.induct)
-case mtchw
-  thus ?case by auto 
-next case mtchv
-  thus ?case by auto 
-next case mtcht
-  thus ?case by auto 
-next case (mtchp s1 p1 e1 s2 p2 e2)
-  then obtain s1' s2' where "matches s1' p1 e1 & matches s2' p2 e2 & s1' @ s2' = s'" by auto
-  hence "s1 @ s2 = s'"
-  proof auto
-    assume "matches s1' p1 e1" 
-       and "matches s2' p2 e2"
-    with mtchp show "s1 @ s2 = s1' @ s2'" by simp
-  qed
-  thus ?case by simp 
-next case (mtchl s p e)
-  hence "matches s' p e" by auto
-  with mtchl show ?case by simp 
-next case (mtchr s p e)
-  hence "matches s' p e" by auto
-  with mtchr show ?case by simp 
-qed
+by (induction s p e arbitrary: s' rule: matches.induct, auto)
 
 lemma [simp]: "matches s p e ==> typecheck env e t ==> types_from_pat p t ts ==> typecheck_subst env s ts"
 by (induction s p e arbitrary: t ts rule: matches.induct, auto)
@@ -203,232 +131,21 @@ proof auto
   ultimately show "typecheck env (apply_subst s e2) t" by simp
 qed 
 
-
-datatype constr = 
-  All
-| CInL type type constr
-| CInR type type constr
-| CTriv
-| CPair constr constr
-
-inductive typecheck_constr :: "constr => type => bool"
-where tcal [simp]: "typecheck_constr All t"
-    | tcil [simp]: "typecheck_constr c t1 ==> typecheck_constr (CInL t1 t2 c) (Sum t1 t2)"
-    | tcir [simp]: "typecheck_constr c t2 ==> typecheck_constr (CInR t1 t2 c) (Sum t1 t2)"
-    | tctr [simp]: "typecheck_constr CTriv Unit"
-    | tcpr [simp]: "typecheck_constr c1 t1 ==> typecheck_constr c2 t2 ==> typecheck_constr (CPair c1 c2) (Prod t1 t2)"
-
-inductive_cases [elim!]: "typecheck_constr All t"
-inductive_cases [elim!]: "typecheck_constr (CInL x y z) t"
-inductive_cases [elim!]: "typecheck_constr (CInR x y z) t"
-inductive_cases [elim!]: "typecheck_constr CTriv t"
-inductive_cases [elim!]: "typecheck_constr (CPair x y) t"
-
-inductive extract_constraint :: "patn => type => constr => bool"       
-where [simp]: "extract_constraint Wild t All"
-    | [simp]: "extract_constraint PVar t All"
-    | [simp]: "extract_constraint PTriv Unit CTriv"
-    | [simp]: "extract_constraint p1 t1 c1 ==> extract_constraint p2 t2 c2 ==> extract_constraint (PPair p1 p2) (Prod t1 t2) (CPair c1 c2)"
-    | [simp]: "extract_constraint p t1 c ==> extract_constraint (PInL p) (Sum t1 t2) (CInL t1 t2 c)"
-    | [simp]: "extract_constraint p t2 c ==> extract_constraint (PInR p) (Sum t1 t2) (CInR t1 t2 c)"
- 
-inductive_cases [elim!]: "extract_constraint Wild t c"
-inductive_cases [elim!]: "extract_constraint PVar t c"
-inductive_cases [elim!]: "extract_constraint PTriv t c"
-inductive_cases [elim!]: "extract_constraint (PPair p1 p2) t c"
-inductive_cases [elim!]: "extract_constraint (PInL p) t c"
-inductive_cases [elim!]: "extract_constraint (PInR p) t c"
-
-lemma [simp]: "extract_constraint PTriv Unit c ==> c = CTriv"
-by (induction PTriv Unit c rule: extract_constraint.induct, simp)
-
-lemma [simp]: "extract_constraint (PPair p1 p2) (Prod t1 t2) c ==> 
-      EX c1 c2. extract_constraint p1 t1 c1 & extract_constraint p2 t2 c2 & c = CPair c1 c2"
-by (induction "PPair p1 p2" "Prod t1 t2" c rule: extract_constraint.induct, simp)
-
-lemma [simp]: "extract_constraint (PInL p) (Sum t1 t2) c ==> 
-      EX c'. extract_constraint p t1 c' & c = CInL t1 t2 c'"
-by (induction "PInL p" "Sum t1 t2" c rule: extract_constraint.induct, simp)
-
-lemma [simp]: "extract_constraint (PInR p) (Sum t1 t2) c ==> 
-      EX c'. extract_constraint p t2 c' & c = CInR t1 t2 c'"
-by (induction "PInR p" "Sum t1 t2" c rule: extract_constraint.induct, simp)
-
-fun get_inls :: "constr list => constr list option"
-where "get_inls [] = Some []"
-    | "get_inls (All # cs) = None"
-    | "get_inls (CInL t1 t2 c # cs) = (case get_inls cs of Some cs' => Some (c # cs') | None => None)"
-    | "get_inls (CInR t1 t2 c # cs) = get_inls cs"
-    | "get_inls (CTriv # cs) = None"
-    | "get_inls (CPair c1 c2 # cs) = None"
-
-fun get_inrs :: "constr list => constr list option"
-where "get_inrs [] = Some []"
-    | "get_inrs (All # cs) = None"
-    | "get_inrs (CInL t1 t2 c # cs) = get_inrs cs"
-    | "get_inrs (CInR t1 t2 c # cs) = (case get_inrs cs of Some cs' => Some (c # cs') | None => None)"
-    | "get_inrs (CTriv # cs) = None"
-    | "get_inrs (CPair c1 c2 # cs) = None"
-
-fun strip_pair_1 :: "constr list => constr list option"
-where "strip_pair_1 [] = Some []"
-    | "strip_pair_1 (All # cs) = (case strip_pair_1 cs of Some cs' => Some (All # cs') | None => None)"
-    | "strip_pair_1 (CInL t1 t2 c # cs) = None"
-    | "strip_pair_1 (CInR t1 t2 c # cs) = None"
-    | "strip_pair_1 (CTriv # cs) = None"
-    | "strip_pair_1 (CPair c1 c2 # cs) = (case strip_pair_1 cs of Some cs' => Some (c1 # cs') | None => None)"
-
-fun strip_pair_2 :: "constr list => constr list option"
-where "strip_pair_2 [] = Some []"
-    | "strip_pair_2 (All # cs) = (case strip_pair_2 cs of Some cs' => Some (All # cs') | None => None)"
-    | "strip_pair_2 (CInL t1 t2 c # cs) = None"
-    | "strip_pair_2 (CInR t1 t2 c # cs) = None"
-    | "strip_pair_2 (CTriv # cs) = None"
-    | "strip_pair_2 (CPair c1 c2 # cs) = (case strip_pair_2 cs of Some cs' => Some (c2 # cs') | None => None)"
-
-lemma [simp]: "Some cs' = get_inls cs ==> list_size size cs' <= list_size size cs"
-proof (induction cs arbitrary: cs' rule: get_inls.induct)
-case 1
-  thus ?case by simp
-next case 2
-  thus ?case by simp
-next case (3 _ _ _ cs)
-  thus ?case
-  proof (cases "get_inls cs")
-  case None
-    with 3 show ?thesis by simp
-  next case (Some ils)
-    with 3 have "list_size size ils <= list_size size cs" by simp
-    with 3 Some show ?thesis by simp
-  qed
-next case (4 _ _ _ cs)
-  hence "list_size size cs' <= list_size size cs" by simp
-  thus ?case by simp
-next case 5
-  thus ?case by simp
-next case 6
-  thus ?case by simp
-qed
-
-lemma [simp]: "Some cs' = get_inls cs ==> list_size size cs' <= Suc (n + list_size size cs)"
-proof -
-  assume "Some cs' = get_inls cs"
-  hence "list_size size cs' <= list_size size cs" by simp
-  thus "list_size size cs' <= Suc (n + list_size size cs)" by simp
-qed
-
-lemma [simp]: "Some cs' = get_inrs cs ==> list_size size cs' <= list_size size cs"
-proof (induction cs arbitrary: cs' rule: get_inrs.induct)
-case 1
-  thus ?case by simp
-next case 2
-  thus ?case by simp
-next case (3 _ _ _ cs)
-  from 3 have "list_size size cs' <= list_size size cs" by simp
-  thus ?case by simp
-next case (4 _ _ _ cs)
-  thus ?case
-  proof (cases "get_inrs cs")
-  case None
-    with 4 show ?thesis by simp
-  next case (Some irs)
-    with 4 have "list_size size irs <= list_size size cs" by simp
-    with 4 Some show ?thesis by simp
-  qed
-next case 5
-  thus ?case by simp
-next case 6
-  thus ?case by simp
-qed
-
-lemma [simp]: "Some cs' = get_inrs cs ==> list_size size cs' <= Suc (n + list_size size cs)"
-proof -
-  assume "Some cs' = get_inrs cs"
-  hence "list_size size cs' <= list_size size cs" by simp
-  thus "list_size size cs' <= Suc (n + list_size size cs)" by simp
-qed
-
-lemma [simp]: "Some cs' = strip_pair_1 cs ==> list_size size cs' <= list_size size cs"
-proof (induction cs arbitrary: cs' rule: strip_pair_1.induct)
-case 1
-  thus ?case by simp
-next case (2 cs)
-  thus ?case
-  proof (cases "strip_pair_1 cs")
-  case None
-    with 2 show ?thesis by simp
-  next case (Some p1s)
-    with 2 have "list_size size p1s <= list_size size cs" by simp
-    with 2 Some show ?thesis by simp
-  qed
-next case 3
-  thus ?case by simp
-next case 4
-  thus ?case by simp
-next case 5
-  thus ?case by simp
-next case (6 _ _ cs)
-  thus ?case
-  proof (cases "strip_pair_1 cs")
-  case None
-    with 6 show ?thesis by simp
-  next case (Some p1s)
-    with 6 have "list_size size p1s <= list_size size cs" by simp
-    with 6 Some show ?thesis by simp
-  qed
-qed
-
-lemma [simp]: "Some cs' = strip_pair_2 cs ==> list_size size cs' <= list_size size cs"
-proof (induction cs arbitrary: cs' rule: strip_pair_2.induct)
-case 1
-  thus ?case by simp
-next case (2 cs)
-  thus ?case
-  proof (cases "strip_pair_2 cs")
-  case None
-    with 2 show ?thesis by simp
-  next case (Some p2s)
-    from 2 Some have "list_size size p2s <= list_size size cs" by simp
-    with 2 Some show ?thesis by simp
-  qed
-next case 3
-  thus ?case by simp
-next case 4
-  thus ?case by simp
-next case 5
-  thus ?case by simp
-next case (6 _ _ cs)
-  thus ?case
-  proof (cases "strip_pair_2 cs")
-  case None
-    with 6 show ?thesis by simp
-  next case (Some p1s)
-    with 6 have "list_size size p1s <= list_size size cs" by simp
-    with 6 Some show ?thesis by simp
-  qed
-qed
-
-fun perfectly_satisfied :: "constr list => bool"
-where "perfectly_satisfied [] = False"
-    | "perfectly_satisfied (All # cs) = (cs = [])"
-    | "perfectly_satisfied (CInL t1 t2 c # cs) = (case (get_inls cs, get_inrs cs) of
-              (Some cls, Some crs) => perfectly_satisfied (c # cls) & perfectly_satisfied crs
-            | _ => False)"
-    | "perfectly_satisfied (CInR t1 t2 c # cs) = (case (get_inls cs, get_inrs cs) of
-              (Some cls, Some crs) => perfectly_satisfied cls & perfectly_satisfied (c # crs)
-            | _ => False)"
-    | "perfectly_satisfied (CTriv # cs) = (cs = [])"
-    | "perfectly_satisfied (CPair c1 c2 # cs) = (case (strip_pair_1 cs, strip_pair_2 cs) of
-              (Some c1s, Some c2s) => perfectly_satisfied (c1 # c1s) & perfectly_satisfied (c2 # c2s)
-            | _ => False)"
+fun perfectly_satisfied :: "type => patn list => bool"
+where "perfectly_satisfied t [] = False"
+    | "perfectly_satisfied t (PInL # ps) = (ps = [PInR] & (EX t1 t2. t = Sum t1 t2))"
+    | "perfectly_satisfied t (PInR # ps) = (ps = [PInL] & (EX t1 t2. t = Sum t1 t2))"
+    | "perfectly_satisfied t (PTriv # cs) = (cs = [] & t = Unit)"
+    | "perfectly_satisfied t (PPair # cs) = (cs = [] & (EX t1 t2. t = Prod t1 t2))"
+    | "perfectly_satisfied t (PZero # cs) = (cs = [PSucc] & t = Nat)"
+    | "perfectly_satisfied t (PSucc # cs) = (cs = [PZero] & t = Nat)"
 
 inductive all_matches_complete :: "expr => bool"
-      and extract_constraints :: "rule list => type => constr list => bool"
-      and extract_constraint_rule :: "rule => type => constr => bool"
+      and extract_patterns :: "rule list => patn list => bool"
+      and extract_pattern :: "rule => patn => bool"
 where [simp]: "all_matches_complete (Var v)" 
     | [simp]: "all_matches_complete Zero"
     | [simp]: "all_matches_complete e ==> all_matches_complete (Succ e)"
-    | [simp]: "all_matches_complete e1 ==> all_matches_complete e2 ==> all_matches_complete e3 ==> all_matches_complete (IsZ e1 e2 e3)"
     | [simp]: "all_matches_complete e ==> all_matches_complete (Lam t' e)"
     | [simp]: "all_matches_complete e1 ==> all_matches_complete e2 ==> all_matches_complete (Ap e1 e2)"
     | [simp]: "all_matches_complete e ==> all_matches_complete (Fix t e)"
@@ -439,15 +156,14 @@ where [simp]: "all_matches_complete (Var v)"
     | [simp]: "all_matches_complete e ==> all_matches_complete (Abort t e)"
     | [simp]: "all_matches_complete e ==> all_matches_complete (InL t1 t2 e)"
     | [simp]: "all_matches_complete e ==> all_matches_complete (InR t1 t2 e)"
-    | [simp]: "all_matches_complete e ==> extract_constraints rs t cs ==> perfectly_satisfied cs ==> all_matches_complete (Match e t rs)"
-    | [simp]: "extract_constraints [] t []"
-    | [simp]: "extract_constraint_rule r t c1 ==> extract_constraints rs t c2 ==> extract_constraints (r # rs) t (c1 # c2)"
-    | [simp]: "extract_constraint p t c ==> all_matches_complete e ==> extract_constraint_rule (Rule p e) t c"
+    | [simp]: "all_matches_complete e ==> extract_patterns rs ps ==> perfectly_satisfied t ps ==> all_matches_complete (Case e t rs)"
+    | [simp]: "extract_patterns [] []"
+    | [simp]: "extract_pattern r p ==> extract_patterns rs ps ==> extract_patterns (r # rs) (p # ps)"
+    | [simp]: "all_matches_complete e ==> extract_pattern (Rule p e) p"
 
 inductive_cases [elim!]: "all_matches_complete (Var x)"
 inductive_cases [elim!]: "all_matches_complete Zero"
 inductive_cases [elim!]: "all_matches_complete (Succ x)"
-inductive_cases [elim!]: "all_matches_complete (IsZ x y z)"
 inductive_cases [elim!]: "all_matches_complete (Lam x y)"
 inductive_cases [elim!]: "all_matches_complete (Ap x y)"
 inductive_cases [elim!]: "all_matches_complete (Fix x y)"
@@ -458,9 +174,9 @@ inductive_cases [elim!]: "all_matches_complete (ProjR v)"
 inductive_cases [elim!]: "all_matches_complete (Abort x y)"
 inductive_cases [elim!]: "all_matches_complete (InL x y z)"
 inductive_cases [elim!]: "all_matches_complete (InR x y z)"
-inductive_cases [elim!]: "all_matches_complete (Match x y z)"
-inductive_cases [elim!]: "extract_constraints [] t c"
-inductive_cases [elim!]: "extract_constraints (x # y) t c"
-inductive_cases [elim!]: "extract_constraint_rule (Rule x y) t c"
+inductive_cases [elim!]: "all_matches_complete (Case x y z)"
+inductive_cases [elim!]: "extract_patterns [] c"
+inductive_cases [elim!]: "extract_patterns (x # y) c"
+inductive_cases [elim!]: "extract_pattern (Rule x y) c"
 
 end
